1.1
$$
L=\frac{1}{2}g_{\alpha\beta}(q)\dot {q}^\alpha\dot {q}^\beta
$$

$$
p &= \sum_{\alpha} \frac{\partial L}{\partial \dot q^\alpha}
\\
&~~~~~~~~~~~~~~~=\frac{1}{2}g_{ij}(\delta_{\alpha}^{i}\dot q^{j}+\dot q^{i}\delta_{\alpha}^{j})
\\
&=g_{\alpha\beta}(q)\dot q^{\beta}
$$

$$
F &= \frac{\partial L}{\partial q^{\alpha}}
\\
&=\frac{1}{2}\frac{\partial g_{ij}(q)}{\partial q^{\alpha}}\dot {q}^i\dot {q}^j
$$

1.2 
$$
\frac{\partial L}{\partial q^{\alpha}} &= \frac{d}{dt}\frac{\partial L}{\partial \dot q^\alpha }
\\
\frac{1}{2}\frac{\partial g_{ij}(q)}{\partial q^{\alpha}}\dot {q}^i\dot {q}^j&=\frac{d}{dt}(g_{\alpha\beta}(q)\dot q^{\beta})
\\
\frac{1}{2}\frac{\partial g_{ij}}{\partial q^{\alpha}}\dot {q}^i\dot {q}^j&=\frac{d}{dt}(g_{\alpha\beta})\dot q^{\beta}+g_{\alpha\beta}\ddot q^{\beta}
\\
\frac{1}{2}\frac{\partial g_{ij}}{\partial q^{\beta}}\dot {q}^i\dot {q}^j&=\frac{\partial (g_{\beta\alpha})}{\partial q^k}\dot q^{k}\dot q^{\alpha} +g_{\beta\alpha}\ddot q^{\alpha}
\\
\frac{1}{2}g^{\alpha\rho}(\frac{\partial g_{\beta\gamma}}{\partial q^{\rho}}\dot {q}^{\beta}\dot {q}^\gamma - 2\frac{\partial g_{\gamma \rho}}{\partial q^\beta}\dot q^{\beta}\dot q^{\gamma})&=\delta_{i}^{\alpha}\ddot q^{i}
\\
\ddot q^{\alpha}+\frac{1}{2}g^{\alpha\rho}(-\frac{\partial g_{\beta\gamma}}{\partial q^{\rho}}\dot {q}^{\beta}\dot {q}^\gamma + \frac{\partial g_{\gamma \rho}}{\partial q^\beta}\dot q^{\beta}\dot q^{\gamma}+\frac{\partial g_{\beta \rho}}{\partial q^\gamma}\dot q^{\beta}\dot q^{\gamma})&=0
\\
Q.E.D
$$


2.1


$$
F_1 &= -k(x_1-x_2-l)
\\
F_2 &= k(x_1-x_2-l)
\\
U(x_1,x_2) &= \frac{1}{2}k(x_1-x_2-l)^2
$$

$$
L=\frac{1}{2}m(\dot x_1^2+\dot x_2^2)-\frac{1}{2}k(x_1-x_2-l)^2
$$

2.2
$$
L=\frac{1}{4}m(4\dot X^2+\dot x^2)-\frac{1}{2}k(x-l)^2
$$
2.3
$$
\frac{\partial L}{\partial x_i} = F_i
$$

$$
\frac{d}{dt}\frac{\partial L}{\partial \dot x_i} = m\ddot x_i
$$

Euler-Lagrange equations:
$$
F_i=m\ddot x_i
\\
0 = m(\ddot x_1+\ddot x_2)
\\
-2k(x_1-x_2-l) = m(\ddot x_1-\ddot x_2)
$$
For $X$ and $x$:
$$
\frac{\partial L}{\partial X} = 0
\\
\frac{\partial L}{\partial x} = -k(x-l)
\\
\frac{d}{dt}\frac{\partial L}{\partial \dot X} = 2m\ddot X
\\
\frac{d}{dt}\frac{\partial L}{\partial \dot x} = \frac{1}{2}m\ddot x
$$
Euler-Lagrange equations:
$$
-2m\ddot X = 0 \rightarrow  \ddot X = 0
\\
-k(x-l)-\frac{1}{2}m\ddot x =0
\\
Q.E.D
$$
